Disable specialized HMAC specs, make test files for SHA and HMAC exemplary, start writing a new parallel Makefile

specs/Spec.HMAC.fst
@@ -22,14 +22,14 @@ let xor_bytes b0 b1 = Spec.Lib.map2 (fun x y -> U8.logxor x y) b0 b1
 
 #reset-options "--max_fuel 0 --z3rlimit 25"
 
-val wrap_key: a:Hash.hash_alg -> key:bytes{Seq.length key < Hash.max_input8 a} -> Tot (okey:bytes{Seq.length okey = Hash.size_block a})
+val wrap_key: a:Hash.Helpers.hash_alg -> key:bytes{Seq.length key < Hash.Helpers.max_input8 a} -> Tot (okey:bytes{Seq.length okey = Hash.Helpers.size_block a})
 let wrap_key a key =
-  if Seq.length key <= Hash.size_block a then
-    let pad = Seq.create ((Hash.size_block a) - (Seq.length key)) 0uy in
+  if Seq.length key <= Hash.Helpers.size_block a then
+    let pad = Seq.create ((Hash.Helpers.size_block a) - (Seq.length key)) 0uy in
     Seq.append key pad
   else begin
-    let nkey = Hash.hash a key in
-    let pad = Seq.create ((Hash.size_block a) - (Hash.size_hash a)) 0uy in
+    let nkey = Hash.Nist.hash a key in
+    let pad = Seq.create ((Hash.Helpers.size_block a) - (Hash.Helpers.size_hash a)) 0uy in
     Seq.append nkey pad
   end
 
@@ -37,18 +37,19 @@ let wrap_key a key =
 #reset-options "--max_fuel 0 --z3rlimit 10"
 
 val hmac_core:
-  a:Hash.hash_alg ->
-  key  :bytes{Seq.length key = Hash.size_block a} ->
-  data :bytes{Seq.length data + Hash.size_block a < Hash.max_input8 a} ->
-  Tot (mac:bytes{Seq.length mac = Hash.size_hash a})
+  a:Hash.Helpers.hash_alg ->
+  key  :bytes{Seq.length key = Hash.Helpers.size_block a} ->
+  data :bytes{Seq.length data + Hash.Helpers.size_block a < Hash.Helpers.max_input8 a} ->
+  Tot (mac:bytes{Seq.length mac = Hash.Helpers.size_hash a})
 
-#reset-options "--max_fuel 0 --z3rlimit 25"
+#reset-options "--max_fuel 0 --z3rlimit 50"
 
 let hmac_core a key data =
 
   (* Define ipad and opad *)
-  let ipad = Seq.create (Hash.size_block a) 0x36uy in
-  let opad = Seq.create (Hash.size_block a) 0x5cuy in
+  let ipad = Seq.create (Hash.Helpers.size_block a) 0x36uy in
+  let opad = Seq.create (Hash.Helpers.size_block a) 0x5cuy in
+  assert (Seq.length opad <= 128);
 
   (* Step 1: the key has the proper length *)
   (* Step 2: xor "result of step 1" with ipad *)
@@ -58,25 +59,34 @@ let hmac_core a key data =
   let s3 = Seq.append s2 data in
 
   (* Step 4: apply H to "result of step 3" *)
-  let s4 = Hash.hash a s3 in
+  let s4 = Hash.Nist.hash a s3 in
+  assert (Seq.length s4 = Hash.Helpers.size_hash a);
+  assert (Seq.length s4 <= 128);
 
   (* Step 5: xor "result of step 1" with opad *)
   let s5 = xor_bytes opad key in
+  assert (Seq.length s5 <= 128);
 
   (* Step 6: append "result of step 4" to "result of step 5" *)
   let s6 = Seq.append s5 s4 in
+  assert (Seq.length s5 <= 256);
+  (
+    let open Spec.Hash.Helpers in
+    match a with
+    | SHA2_224 | SHA2_256 -> assert_norm (256 <= pow2 61)
+    | SHA2_384 | SHA2_512 -> assert_norm (256 <= pow2 125));
 
   (* Step 7: apply H to "result of step 6" *)
-  Hash.hash a s6
+  Hash.Nist.hash a s6
 
 
 #reset-options "--max_fuel 0 --z3rlimit 10"
 
 val hmac:
-  a    :Hash.hash_alg ->
-  key  :bytes{Seq.length key < Hash.max_input8 a} ->
-  data :bytes{Seq.length data + Hash.size_block a < Hash.max_input8 a} ->
-  Tot (mac:bytes{Seq.length mac = Hash.size_hash a})
+  a    :Hash.Helpers.hash_alg ->
+  key  :bytes{Seq.length key < Hash.Helpers.max_input8 a} ->
+  data :bytes{Seq.length data + Hash.Helpers.size_block a < Hash.Helpers.max_input8 a} ->
+  Tot (mac:bytes{Seq.length mac = Hash.Helpers.size_hash a})
 
 #reset-options "--max_fuel 0 --z3rlimit 25"
 
